

CMPUT 567: Machine Learning 2

Keven Qiu
Instructor: Martha White

Contents

1	Generalization Error	1
1.1	Bias and Variance for Linear Regression	2
1.2	ℓ_2 -Regularization	3
1.3	Better Generalization Error	3
2	Optimization	4
2.1	Comparisons	6
3	Generalized Linear Models	7
3.1	Poisson Example	7
3.2	General Form for GLM	8
3.3	GLM Update	8
3.4	Multinomial Logistic Regression	9
3.5	Add Regularization to GLM	10
4	Constrained Optimization With Proximal Methods	11
4.1	Proximal Gradient Descent	11
4.1.1	Box Constraints	11
4.1.2	ℓ_1 -Regularization	12
4.1.3	Linear Regression	12

1 Generalization Error

The generalization error for a given f , with squared error is

$$E_{x,y}[(f(X) - Y)^2] = \underbrace{E[(f(X) - f^*(X))^2]}_{\text{reducible error}} + \underbrace{E[(f^*(X) - Y)^2]}_{\text{irreducible error}}$$

where $f^*(x) = E[Y|x]$ and the irreducible error is $E_x[\text{Var}(Y|X)]$.

Bias and variance is about the function class \mathcal{F} (and algorithm, i.e. objective and optimizer).

$$f_{\mathcal{D}} = \text{Alg}(\mathcal{D})$$

where $\mathcal{D} \sim \underbrace{p(x_1, y_1)p(x_2, y_2) \cdots p(x_n, y_n)}_{p(\mathcal{D})}$. Then

$$E_{\mathcal{D}}[GE(f_{\mathcal{D}})] = E_{\mathcal{D}}[\underbrace{\text{reducible error}(f_{\mathcal{D}})}_{\text{bias}^2 + \text{variance}}] + \text{irreducible error}$$

Note there are two variances: the irreducible error and the variance of our function f .

For one x :

$$\begin{aligned} E_{\mathcal{D}}[(f_{\mathcal{D}}(x) - f^*(x))^2] &= E_{\mathcal{D}}[\underbrace{(f_{\mathcal{D}}(x) - E_{\mathcal{D}}[f_{\mathcal{D}}(x)])}_a + \underbrace{(E_{\mathcal{D}}[f_{\mathcal{D}}(x)] - f^*(x))}_b]^2 \\ &= \underbrace{b^2}_{\text{bias}^2} + \underbrace{a^2}_{\text{variance}} + 2 \underbrace{E_{\mathcal{D}}[f_{\mathcal{D}}(x) - E_{\mathcal{D}}[f_{\mathcal{D}}(x)]]}_{=0} b \\ &= (E_{\mathcal{D}}[f_{\mathcal{D}}(x)] - f^*(x))^2 + \text{Var}_{\mathcal{D}}(f_{\mathcal{D}}(x)) \end{aligned}$$

If we can represent f^* (high model complexity), then $E_{\mathcal{D}}[f_{\mathcal{D}}(x)] \approx f^*(x)$ for all x .

1.1 Bias and Variance for Linear Regression

With nonlinear representation Φ , we have by SVD

$$\Phi = U\Sigma V^T \in \mathbb{R}^{n \times p}$$

where $U = [u_1, \dots, u_n]$, with left singular vectors $u_j \in \mathbb{R}^{n \times 1}$ and $V = [v_1, \dots, v_p]$, with right singular vectors $v_j \in \mathbb{R}^{p \times 1}$, and $\Sigma \in \mathbb{R}^{n \times p}$.

We consider thin SVD, where we consider only the first p rows/columns.

$$\Sigma = \begin{bmatrix} \sigma_1 & \cdots & 0 \\ 0 & \ddots & 0 \\ 0 & \cdots & \sigma_p \\ \vdots & \vdots & \vdots \\ 0 & \cdots & 0 \end{bmatrix}, \Sigma_p = \text{diag}(\sigma_1, \dots, \sigma_p), U_p = [u_1, \dots, u_p]$$

since $U\Sigma = U_p\Sigma_p$. Note that $\Sigma^T\Sigma = \Sigma_p^2$.

$$\begin{aligned} \Phi^T\Phi &= V\Sigma^T U^T U\Sigma V^T \\ &= V\Sigma^T\Sigma V^T \\ &= V\Sigma_p^2 V^T \\ \mathbf{w} &= (\Phi^T\Phi)^{-1}\Phi^T y \\ &= V\Sigma_p^{-2} V^T V\Sigma_p U_p^T y \\ &= V\Sigma_p^{-1} U_p^T y \\ &= \sum_{j=1}^p \frac{u_j^T y}{\sigma_j} v_j \end{aligned}$$

Note that for this, all singular values must be nonzero/positive. $\Phi^t = V\Sigma_p^{-1}U_p^T$ is known as the pseudoinverse of Φ .

If Φ has lower rank $r < p$, i.e. $\sigma_1, \dots, \sigma_r > 0, \sigma_{r+1}, \dots, \sigma_p = 0$, then $\Phi^t = V_r \Sigma_r^{-1} U_r^T$ where $V_r = [v_1, \dots, v_r]$.

Notice that \mathbf{w} is sensitive to small singular values since we divide by them. Reasons why σ_j can be small:

- linearly correlated features (one dimension might not have anything)
- insufficient data

1.2 ℓ_2 -Regularization

For linear regression, the MLE is $p(y|x) = \mathcal{N}(\phi w, \sigma^2)$. MAP with Gaussian prior is $-\ln p(w_j) = \text{constant} + \frac{\lambda}{2\sigma^2} w_j^2$.

$$c(w) = \frac{1}{2} \|\Phi w - y\|_2^2 + \frac{\lambda}{2} \|w\|_2^2 \implies (\Phi^T \Phi + \lambda I)w = \Phi^T y \implies w = (\Phi^T \Phi + \lambda I)^{-1} \Phi^T y$$

Using SVD $\Phi^T \Phi + \lambda I = V(\Sigma_p^2 + \lambda I)V^T$,

$$w_{MAP} = V(\Sigma_p^2 + \lambda I)^{-1} U_p^T y = \sum_{j=1}^p \frac{\sigma_j}{\sigma_j^2 + \lambda} (u_j^T y) v_j$$

As long as large λ , the fraction does not blow up like it did without ℓ_2 -regularization.

1.3 Better Generalization Error

Realizable setting: $y \sim \mathcal{N}(\Phi w^*, \sigma^2)$ for some w^* and $f^* \in \mathcal{F}$ (f^* is in function class).

Let $w(\mathcal{D})$ be our estimator.

$$MSE(w(\mathcal{D})) = E_{\mathcal{D}} \left[\sum_{j=1}^p (w_j(\mathcal{D}) - w_j^*)^2 \right] = \sum_{j=1}^p (E[w_j(\mathcal{D})] - w_j^*)^2 + \sum_{j=1}^p \text{Var}(w_j(\mathcal{D}))$$

Notice $y = \phi w^* + \varepsilon$ where $\varepsilon \sim \mathcal{N}(0, \sigma^2)$. For MLE,

$$\begin{aligned} E[w_{MLE}(\mathcal{D})] &= E[(\Phi^T \Phi)^{-1} \Phi^T y] \\ &= E[(\Phi^T \Phi)^{-1} \Phi^T (\Phi w^* + \varepsilon)] \\ &= E[(\Phi^T \Phi)^{-1} (\Phi^T \Phi) w^*] + \underbrace{E[(\Phi^T \Phi)^{-1} \Phi^T] E[\varepsilon]}_{=0} \\ &= w^* \end{aligned}$$

This is unbiased as it equals w^* . For MLE variance,

$$\sum_{j=1}^p \text{Var}(w_{MLE}(\mathcal{D})) = \sigma^2 E \left[\sum_{j=1}^p \sigma_j^{-2} \right]$$

where first σ^2 is variance, not singular value. This can be very big if σ_p is often small.

For MAP,

$$E[w_{MAP}(\mathcal{D})] = E[(\Phi^T \Phi + \lambda I)^{-1} \Phi^T (\Phi w^* + \varepsilon)] \neq w^*$$

so this is biased as λ increases.

$$\sum_{j=1}^p \text{Var}(w_{MAP}(\mathcal{D})) = \sigma^2 E \left[\sum_{j=1}^p \frac{\sigma_j^2}{(\sigma_j^2 + \lambda)^2} \right]$$

This is not very big if λ is large.

Non-realizable: $y = \mathcal{N}(f^*(x), \sigma^2)$, but $f^* \notin \mathcal{F}$. w_{MLE} is also biased.

Note about n : We can stick a $\frac{1}{n}$ in front of $\Phi^T \Phi$ to act like an average over outerproducts. Note $\frac{1}{n} \Phi^T \Phi = E[\Phi^T \Phi]$.

Without normalization, $\sigma_j^2 \rightarrow \infty$ as $n \rightarrow \infty$. With normalization $\frac{1}{n} \sigma_j^2 \rightarrow$ singular values for $E[\Phi^T \Phi]$.

$\sum_{j=1}^p \sigma_j^{-2} \rightarrow 0$ as $n \rightarrow \infty$, so $\text{Var}(w_{MLE}(\mathcal{D})) \rightarrow 0$ as $n \rightarrow \infty$.

Multiple outputs: $y \in \mathbb{R}^m$, $\phi(x)W \approx y$.

$$Y = \begin{bmatrix} y_{11} & \cdots & y_{1m} \\ \vdots & \ddots & \vdots \\ y_{n1} & \cdots & y_{nm} \end{bmatrix} = [\mathbf{y}_1 \quad \cdots \quad \mathbf{y}_m]$$

where $\mathbf{y}_i \in \mathbb{R}^n$. So

$$\mathbf{w} = \Phi^t Y = [\Phi^t \mathbf{y}_1 \quad \cdots \quad \Phi^t \mathbf{y}_m]$$

2 Optimization

Find

$$\min_{w \in \mathbb{R}^p} c(w)$$

For example, $c(w) = \frac{1}{n} \sum_{i=1}^n c_i(w)$, linear regression $c_i(w) = \frac{1}{2}(\phi(x_i)w - y_i)^2$ or logistic regression $c_i(w) = -y_i \ln f_w(x_i) - (1 - y_i) \ln(1 - f_w(x_i))$.

1. Find a stationary point w_0 , $\nabla c(w_0) = 0$.
2. Check type using second derivative test ($c'_i(w_t) < 0, > 0, = 0$).

In p -dimensions, the **Hessian** matrix $H_{c(w_t)} \in \mathbb{R}^{p \times p}$, where

$$H_{c(w)}[i, j] = \frac{\partial^2 c}{\partial w_i \partial w_j}(w)$$

$$\text{E.g. } c(w) = \frac{1}{2}(w_1 + xw_2 - y)^2, \nabla c(w) = \begin{bmatrix} (w_1 + xw_2 - y) \\ (w_1 + xw_2 - y)x \end{bmatrix} = \begin{bmatrix} \frac{\partial c}{\partial w_1}(w) \\ \frac{\partial c}{\partial w_2}(w) \end{bmatrix}.$$

$$H_{c(w)} = \begin{bmatrix} \frac{\partial}{\partial w_1} \frac{\partial}{\partial w_1} c(w) & \frac{\partial}{\partial w_1} \frac{\partial}{\partial w_2} c(w) \\ \frac{\partial}{\partial w_2} \frac{\partial}{\partial w_1} c(w) & \frac{\partial}{\partial w_2} \frac{\partial}{\partial w_2} c(w) \end{bmatrix} = \begin{bmatrix} 1 & x \\ x & x^2 \end{bmatrix}$$

For $(x = 0.1, y = 2)$ and $w_0 = (0, 0)$,

$$\nabla c(w) = \begin{bmatrix} -2 \\ -0.2 \end{bmatrix}, H_{c(w_0)} = \begin{bmatrix} 1 & 0.1 \\ 0.1 & 0.01 \end{bmatrix}$$

The eigenvalues of $H_{c(w_0)}$ are $\lambda_1 \approx 1, \lambda_2 = 0$. So we get a concave up in one direction, and flat in the other direction (a taco shape).

E.g. $c(w) = \frac{1}{2}(w_1 + x_1 w_2 - y_1)^2 + \frac{1}{2}(w_1 + x_2 w_2 - y_2)^2$. At $(x_1 = 0.1, y_1 = 2)$ and $(x_2 = -0.3, y_2 = -1)$,

$$H_{c(w_0)} = \begin{bmatrix} 2 & -0.2 \\ -0.2 & 0.1 \end{bmatrix}$$

for $w_0 = (0, 0)$. The eigenvalues are $\lambda_1 = 6.5, \lambda_2 = 0.08$.

Better Steps: $H_{c(w)}^{-1}$ is a matrix stepsize. The second-order method is

$$w_{t+1} = w_t - H_{c(w_t)}^{-1} \nabla c(w_t)$$

The scalar version was $w_{t+1} = w_t - \frac{1}{c''(w_t)} \cdot c'(w_t)$.

Using eigenvalue decomposition, $H_{c(w_t)}^{-1} \nabla c(w_t) = U \Lambda^{-1} \underbrace{U^T \nabla c(w_t)}_{\tilde{g}_t}$. This shows that the step is

inversely proportional to curvature magnitude (λ_i 's). One step size could be bad, since in regular gradient descent uses stepsize η , so Hessian allows us not to step too much on steep surfaces and more on flat surfaces.

Computational issues: Computing $H_{c(w)}^{-1}$ is $O(p^2 n)$ for linear regression. This is because $H_{c(w)} = \frac{1}{n} \sum_{i=1}^n H_{c_i(w)}$, where $H_{c_i(w)}$ takes $O(p^2)$ and you sum n times. Computing the inverse is $O(p^3)$, but for $p < n$, $p^3 < p^2 n$, so $O(p^2 n)$ overall.

An alternative is to use a vector of stepsizes $\eta_t \in \mathbb{R}^p$. So

$$H_{c(w_t)}^{-1} \approx \text{diag}(\eta_{t,1}, \eta_{t,2}, \dots, \eta_{t,p})$$

and the update is

$$w_{t+1} = w_t - \eta_t \overset{\text{element-wise product}}{\cdot} \nabla c(w_t)$$

We do not use a fixed $\eta \in \mathbb{R}^p$. We use vector stepsizes, that change with time.

Definition 2.1: Adagrad

$$\eta_{t,j} = (1 + \bar{g}_{t,j})^{-1/2}$$

where $\bar{g}_{t,j} = \bar{g}_{t-1,j} + g_{t,j}^2$ and $\bar{g}_0 = 0$.

This has nice theory, but in practice, stepsizes shrink too much since we have a monotonic decrease in stepsize.

An intuitive modification is to take an exponential average of $g_{t,j}^2$, which leads to RMSProp.

Definition 2.2: RMSProp

$$v_{t,j} = (1 - \beta)g_{t,j}^2 + \beta v_{t-1,j}, \beta > 0$$

$$\eta_{t,j} = \frac{\eta}{\sqrt{v_{t,j} + \varepsilon}} = \eta(v_{t,j} + \varepsilon)^{-1/2}$$

Also add **momentum**: with fixed stepsize η ,

$$w_{t+1} = w_t - \eta m_{t+1}, m_{t+1} = g_t + \beta_2 m_t, \beta_2 > 0$$

An alternate form is

$$w_{t+1} = w_t - \eta g_t + \beta(w_t - w_{t-1})$$

Definition 2.3: Adam

Puts RMSProp and momentum together with extra modification.

There is a bias correct for $v_{0,j} = 0$. There is an exponential average in momentum $m_{t+1} = (1 - \beta_2)g_t + \beta_2 m_t$. The last modification is

$$\text{Adam's } \frac{1}{\sqrt{v_{t,j} + \varepsilon}} \text{ vs. RMSProp's } \frac{1}{\sqrt{v_{t,j} + \varepsilon}}$$

2.1 Comparisons

Second-order updates takes $O(p^2n)$ per iteration and gradient descent takes $O(pn)$ per iteration.

Definition 2.4: Stochastic Gradient Descent (SGD)

Randomly pick $\mathcal{B}_t \subseteq \{1, \dots, n\}$ with $|\mathcal{B}_t| = b$, the gradient $\hat{g}_t = \frac{1}{b} \sum_{i \in \mathcal{B}_t} \nabla c_i(w_t)$,

$$w_{t+1} = w_t - \eta_t \hat{g}_t = w_t - \underbrace{\eta_t \nabla c(w_t)}_{\text{GD}} + \underbrace{\eta_t \left(\nabla c(w_t) - \frac{1}{b} \sum_{i \in \mathcal{B}} \nabla c_i(w_t) \right)}_{\text{noise term, expected value}=0}$$

The runtime is $O(pb)$.

This is much faster than $O(pn)$ for GD. $\hat{g}_t \approx g_t = \frac{1}{n} \sum_{i=1}^n \nabla c_i(w_t) = \nabla c(w)$.

How do we pick between 2nd order GD (Newton's method), 1st order GD, SGD? In terms of computations, cost = # of iterations \times compute per iteration. The convergence criterion is

$$\|\nabla c(w_t)\|_2^2 \leq \varepsilon$$

for $\varepsilon > 0$.

For now, assume $\|\nabla c(w)\| \leq L$ for any w .

- GD with fixed stepsize $\eta > 0$: After t updates/iterations:

$$\|\nabla c(w_t)\|_2^2 \leq \frac{2L}{t} \left(\underbrace{c(w_0) - c(w^*)}_{\text{how far start was from optimal}} \right)$$

So, $t \geq 2L/\varepsilon \cdot (c(w_0) - c(w^*))$ or $t = O(1/\varepsilon)$. For $\varepsilon = 0.1$, then $t = 1/\varepsilon = 10$. For $\varepsilon = 0.01$, then $t = 100$. For $t = O(1/\varepsilon)$, this is sublinear convergence. Progress slows down.

GD takes $O(np/\varepsilon)$ compute to converge.

- 2nd-Order GD: $t = O(\log(1/\varepsilon))$. For $\varepsilon = 0.1$, $t = 1$. For $\varepsilon = 0.01$, $t = 2$.

2nd-order GD takes $O(np^2 \log(1/\varepsilon))$.

When is $np^2 \log(1/\varepsilon) < np/\varepsilon \implies p^2 \log(1/\varepsilon) < p/\varepsilon$, i.e. when is 2nd-order GD better than GD? For $p = 10, \varepsilon = 0.01$, $20 < 100$. For $p = 100, \varepsilon = 0.01$, $200 > 100$. So when we have a small number of weights/ p , 2nd-order is faster.

- SGD vs. GD: SGD uses minibatches \mathcal{B} of size b . If constant $\eta > 0$, almost the same convergence as GD. The convergence is

$$O\left(\frac{1}{t}\right) + \frac{L\sigma_{\mathcal{B}}^2\eta}{2}$$

$\sigma_{\mathcal{B}}^2$ is related to noisiness of gradient.

If $\eta_t = \eta/\sqrt{t}$, then $O(1/\sqrt{t})$, the oscillations eventually decay.

How can we keep $O(1/t)$ SGD convergence rate, but still reduce error term to 0? You can start with small minibatches, and increase them over time.

3 Generalized Linear Models

For classification, we had a Bernoulli distribution, $y \in \{0, 1\}$, and we learned $p(y = 1|x) = \sigma(\phi w)$. For linear regression, we had a Gaussian distribution, $y \in \mathbb{R}$, and we learned $p(y|x) = \mathcal{N}(\phi w, \sigma^2)$, where $\phi w = E[Y|x]$.

Others include Poisson distribution or multinomial distribution. $p(y|x)$ is an exponential family distribution.

3.1 Poisson Example

Imagine $y \in \{0, 1, \dots\}$ such as number of accidents in a factory, conditioned on factory info x . The pmf for Poisson is

$$p(z) = \frac{\lambda^z \exp(-\lambda)}{z!}$$

for $\lambda > 0$ is mean of Poisson distribution.

$$p(y|x) = \frac{\lambda(x)^y \exp(-\lambda(x))}{y!}$$

Our goal is to learn $\lambda(x)$.

First attempt: $\lambda(x) = \phi w$, i.e. linear regression. This does not work since $\phi w < 0$, but $\lambda > 0$.

Second attempt: $\lambda(x) = \exp(\phi w)$. Getting closer.

3.2 General Form for GLM

Definition 3.1: General Form of Generalized Linear Models

$$p(y|x) = \exp(\phi w y - a(\phi w) + b(y))$$

where transfer function $g(\phi w) = a'(\phi w)$ and $E[Y|x] = g(\phi w)$.

E.g. Gaussian $a(\phi w) = \frac{1}{2}(\phi w)^2$, $g(\phi w) = a'(\phi w) = \phi w$.

$a(\theta) = \frac{1}{2}\theta^2$, $a'(\theta) = \theta$, $b(y) = -\frac{1}{2}y^2 + \ln \frac{1}{\sqrt{2\pi}}$. The general form is

$$\begin{aligned} p(y|x) &= \exp\left(\phi w y - \frac{1}{2}(\phi w)^2 - \frac{1}{2}y^2 + \ln \frac{1}{\sqrt{2\pi}}\right) \\ &= \exp\left(-\frac{1}{2}(\phi w - y)^2\right) \exp\left(\ln \frac{1}{\sqrt{2\pi}}\right) \\ &= \frac{1}{\sqrt{2\pi}} \exp\left(-\frac{1}{2}(\phi w - y)^2\right) \end{aligned}$$

E.g. Bernoulli $a'(\theta) = \sigma(\theta)$, $g(\phi w) = \sigma(\phi w)$.

E.g. Poisson $a(\theta) = \exp(\theta)$, $a'(\theta) = \exp(\theta) = g(\theta)$, $b(y) = -\ln y!$. The general form is

$$\begin{aligned} p(y|x) &= \exp((\phi w)y - \exp(\phi w) - \ln y!) \\ &= \exp(\phi w y) \exp(-\exp(\phi w)) \exp(-\ln y!) \\ &= \frac{\exp(\phi w)^y \exp(-\exp(\phi w))}{y!} & (e^{ab} = (e^a)^b) \\ &= \frac{\lambda(x)^y \exp(-\lambda(x))}{y!} & (\lambda(x) = g(\phi w) = \exp(\phi w)) \end{aligned}$$

3.3 GLM Update

Given a dataset $\mathcal{D} = \{(x_i, y_i)\}_{i=1}^n$, $\phi_i = \phi(x_i)$,

$$c_i(w) = -\ln p(y_i|x_i, w) = -\ln \exp(\phi_i w y_i - a(\phi_i w) + b(y_i)) = -(\phi_i w) y_i + a(\phi_i w) + \text{constant}$$

The gradient is

$$\nabla c_i(w) = -y_i \phi_i^T + a'(\phi_i w) \phi_i^T = (a'(\phi_i w) - y_i) \phi_i^T = (\underbrace{g(\phi_i w)}_{\text{prediction}} - y_i) \phi_i^T$$

For linear regression, $(\phi_i w - y_i) \phi_i^T$, for logistic regression, $(\sigma(\phi_i w) - y_i) \phi_i^T$, and for Poisson regression, $(\exp(\phi_i w) - y_i) \phi_i^T$.

Recap on the three GLMs:

- **Linear regression:** For $y \in \mathbb{R}$

$$g(\phi w) = \phi w \approx E[Y|x]$$

Predict with $g(\phi w)$.

- **Logistic regression:** For $y \in \{0, 1\}$

$$g(\phi w) = \sigma(\phi w) \approx E[Y|x]$$

Predict $\mathbf{1}(\sigma(\phi w) > 0.5) \approx p(y = 1|x) = E[Y|x]$.

- **Poisson regression:** For $y \in \{0, 1, 2, \dots\}$

$$g(\phi w) = \exp(\phi w) \approx E[Y|x]$$

Predict $g(\phi w)$ or mode of $\text{Poisson}(\lambda = g(\phi w))$.

3.4 Multinomial Logistic Regression

This is another GLM and is multiclass classification. Given an input $x \in \mathbb{R}^{1 \times d}$ and output $y \in \mathbb{R}^{1 \times m} \in \{e_1^T, e_2^T, \dots, e_m^T\}$ where e_i^T is the row elementary vector with 1 in the i th coordinate for each class. For matrices, we have $X \in \mathbb{R}^{n \times d}$ and $Y = (y_1, \dots, y_n)^T \in \mathbb{R}^{n \times m}$.

$$p(y = [y_1, \dots, y_m]) = p(y_1 = 1)^{y_1} p(y_2 = 1)^{y_2} \dots p(y_m = 1)^{y_m} = \alpha_1^{y_1} \alpha_2^{y_2} \dots \alpha_m^{y_m}$$

where $\sum_{k=1}^m \alpha_k = 1$ and $\alpha_k \geq 0$.

E.g. $p(y = [0, 1, 0, \dots, 0]) = \alpha_1^0 \alpha_2^1 \alpha_3^0 \dots \alpha_m^0 = 0 = \alpha_2$.

In general, we want the probability given x ,

$$p(y = [y_1, \dots, y_m]) = \alpha_1(x)^{y_1} \dots \alpha_m(x)^{y_m}$$

We cannot have a transfer function $\alpha_k(x) = \sigma(\phi w_k)$ as the probabilities may not sum to 1. We can normalize so the sum is 1, this leads to the softmax function.

The transfer function g is

$$\text{softmax}(\phi W) = \left[\underbrace{\frac{\exp(\phi w_1)}{\sum_{k=1}^m \exp(\phi w_k)}}_{\alpha_1(x)} \quad \dots \quad \underbrace{\frac{\exp(\phi w_m)}{\sum_{k=1}^m \exp(\phi w_k)}}_{\alpha_m(x)} \right]$$

where $\phi \in \mathbb{R}^{1 \times p}$ and $W \in \mathbb{R}^{p \times m}$.

For each x_i ,

$$p_i = \text{softmax}(\phi_i W) \in \mathbb{R}^{1 \times m}$$

So, $p_{i1} = p(y_i = 1|x_i)$, $p_{i2} = p(y_i = 2|x_i)$, and so forth.

E.g. $m = 4$, $p_i = [0.1, 0.4, 0.3, 0.2]$, $y_i = [0, 0, 1, 0]$. Select the class

$$\hat{y}_i = \arg \max_{k \in \{1, \dots, m\}} \text{softmax}(\phi_i W) = [0, 1, 0, 0] \text{ or } 2$$

even though actual y_i is 3.

Why do we get $p_i = [0.1, 0.4, 0.3, 0.2]$, rather than $p_i = [0, 0.99, 0, 0.01]$?

- The true $p(y|x_i) = p_i$ (uncertainty, irreducible error).
- Could be insufficient data or optimization (uncertainty estimation).

GLM Update

$$c_i(W) = -\ln p(y_i|x_i), \frac{\partial c_i(W)}{\partial W_{jk}} = (p_{ik} - y_{ik})\phi_{ij}$$

For all features,

$$\frac{\partial c_i(W)}{\partial W_{:k}} = (p_{ik} - y_{ik})\phi_i^T$$

For the entire matrix,

$$\frac{\partial c_i(W)}{\partial W} = [\phi_i^T(p_{i1} - y_{i1}), \dots, \phi_i^T(p_{im} - y_{im})] = \phi_i^T(p_i - y_i) = g_i \in \mathbb{R}^{p \times m}$$

The update is

$$W_{t+1} = W_t - \eta_t \circ g_t$$

where \circ is element-wise product.

An extra detail: we only need to learn $w_1, \dots, w_{m-1} \in \mathbb{R}^{p \times 1}$ since we can infer $p(y_m = 1|x) = 1 - \sum_{k=1}^{m-1} p(y_k = 1|x)$. We can pivot with $w_m = 0$ and only update w_1, \dots, w_{m-1} . This is w_m extra degrees of freedom.

Connection to Logistic Regression: For $m = 2$, $y_{LR} = 1 \implies y = [1, 0]$ and $y_{LR} = 0 \implies y = [0, 1]$. $w_1 = w$, $w_2 = 0$. Thus, we learn one weight vector $w_1 = w$ and pivot over w_2 .

$$p(y_{LR} = 1|x) = \frac{\exp(\phi w_1)}{\exp(\phi w_1) + \exp(\phi w_2)} = \frac{\exp(\phi w)}{\exp(\phi w) + 1} = \sigma(\phi w) = \frac{1}{1 + \exp(-\phi w)}$$

We can learn w_2 with

$$p(y_{LR} = 0|x) = p(y = [0, 1]|x) = 1 - \sigma(\phi w)$$

3.5 Add Regularization to GLM

ℓ_2 -Regularization:

$$\frac{1}{n} \sum_{i=1}^n c_i(w) + \frac{\lambda}{2} \|w\|_2^2$$

where the first summand is the MLE part ($-\ln p(y|x)$) and the second summand is the Gaussian prior, so the entire thing is MAP.

Update: $w_{t+1} = w_t - \eta_t \circ \phi_i^T(p_i - y_i) - \lambda \eta_t \circ w_t$.

ℓ_1 -Regularization:

$$\frac{1}{n} \sum_{i=1}^n c_i(w) + \lambda \|w\|_1$$

where $\|w\|_1 = \sum_{j=1}^p |w_j|$. ℓ_1 is a V-shape function, so it has a stronger preference to reach $w = 0$. ℓ_2 has a strong preference for small w .

4 Constrained Optimization With Proximal Methods

4.1 Proximal Gradient Descent

We are given the optimization problem

$$\min_{w \in \mathbb{R}^p} c(w) + r(w)$$

where c is smooth (differentiable everywhere) and r is non-smooth.

E.g. ℓ_1 -regularizer $r(w) = \lambda \|w\|_1$. This is not differentiable at $w = 0$. For gradient descent, it will keep jumping back and forth between both sides, since the gradients do not get smaller.

E.g. Constraints $w \in [-1, 1]^p$,

$$r_{\text{box}}(w) = \begin{cases} 0 & \text{if } w \in [-1, 1]^p \\ \infty & \text{otherwise} \end{cases}$$

Recall gradient descent: Local Taylor series approximation

$$c(w) \approx \hat{c}_t(w) = c(w_t) + \nabla c(w_t)^T (w - w_t) + \frac{1}{2\eta_t} \|w - w_t\|_2^2$$

Then,

$$w_{t+1} = \arg \min_{w \in \mathbb{R}^p} \hat{c}_t(w), \nabla \hat{c}_t(w) = 0 \implies w_{t+1} = w_t - \eta_t \nabla c(w_t)$$

Now, we have a non-smooth $r(w)$, so

$$w_{t+1} = \arg \min_{w \in \mathbb{R}^p} \hat{c}_t(w) + r(w)$$

Using algebraic manipulation, we can get a equivalent optimization problem:

$$w_{t+1} = \arg \min_{w \in \mathbb{R}^p} \frac{1}{2} \left\| w - \underbrace{(w_t - \eta_t \nabla c(w_t))}_{\text{usual GD outcome}} \right\|_2^2 + \eta_t r(w)$$

Algorithm: Proximal Gradient Descent

1. $\tilde{w}_{t+1} = w_t - \eta_t \nabla c(w_t)$.
2. $w_{t+1} = \text{prox}_{\eta_t r}(w) = \arg \min_{w \in \mathbb{R}^p} \frac{1}{2} \|w - \tilde{w}_{t+1}\|_2^2 + \eta_t r(w)$ (proximal operator).

4.1.1 Box Constraints

For

$$r_{\text{box}}(w_j) = \begin{cases} 0 & w_j \in [a, b] \\ \infty & \text{otherwise} \end{cases}$$

we have the proximal operator

$$\text{prox}_{\eta_t r_{\text{box}}}(v) = \begin{cases} a & \text{if } v < a \\ v & \text{if } v \in [a, b] \\ b & \text{if } v > b \end{cases}$$

Derivation: Minimization is separable.

$$\frac{1}{2} \sum_{i=1}^p (w_j - \tilde{w}_{t+1,j})^2 + \eta_t \sum_{j=1}^p r_{\text{box}}(w_j)$$

Independently,

$$\min_{w_j \in \mathbb{R}} \frac{1}{2} (w_j - \tilde{w}_{t+1,j})^2 + \eta_t r_{\text{box}}(w_j)$$

The solution w is the following:

- If $\tilde{w}_{t+1,j} \in [a, b]$, then $w_j = \tilde{w}_{t+1,j}$.
- If $\tilde{w}_{t+1,j} < a$, then $w_j = a$.
- If $\tilde{w}_{t+1,j} > b$, then $w_j = b$.

4.1.2 ℓ_1 -Regularization

For $r(w) = \lambda \|w\|_1 = \lambda \ell_1(w)$,

$$\text{prox}_{\eta_t \lambda \ell_1}(\tilde{w}_{t+1,j}) = \begin{cases} \tilde{w}_{t+1,j} - \eta_t \lambda & \text{if } \tilde{w}_{t+1,j} > \eta_t \lambda \\ 0 & \text{if } |\tilde{w}_{t+1,j}| \leq \eta_t \lambda \\ \tilde{w}_{t+1,j} + \eta_t \lambda & \text{if } \tilde{w}_{t+1,j} < -\eta_t \lambda \end{cases}$$

4.1.3 Linear Regression

The first step is $\tilde{w}_{t+1} = w_t - \eta_t (\phi_i w_t - y_i) \phi_i^T$. The second step is

$$w_{t+1} = \text{prox}_{\eta_t \lambda \ell_1}(\tilde{w}_{t+1})$$

element-wise.